can extract ocaml

ocaml/generated/extract.ml
@@ -1,0 +1,748 @@
+
+type nat =
+| O
+| S of nat
+
+type comparison =
+| Eq
+| Lt
+| Gt
+
+(** val compOpp : comparison -> comparison **)
+
+let compOpp = function
+| Eq -> Eq
+| Lt -> Gt
+| Gt -> Lt
+
+module Coq__1 = struct
+ (** val add : nat -> nat -> nat **)
+ let rec add n m =
+   match n with
+   | O -> m
+   | S p -> S (add p m)
+end
+include Coq__1
+
+(** val eqb : nat -> nat -> bool **)
+
+let rec eqb n m =
+  match n with
+  | O -> (match m with
+          | O -> true
+          | S _ -> false)
+  | S n' -> (match m with
+             | O -> false
+             | S m' -> eqb n' m')
+
+(** val map : ('a1 -> 'a2) -> 'a1 list -> 'a2 list **)
+
+let rec map f = function
+| [] -> []
+| a :: t -> (f a) :: (map f t)
+
+(** val fold_left : ('a1 -> 'a2 -> 'a1) -> 'a2 list -> 'a1 -> 'a1 **)
+
+let rec fold_left f l a0 =
+  match l with
+  | [] -> a0
+  | b :: t -> fold_left f t (f a0 b)
+
+(** val seq : nat -> nat -> nat list **)
+
+let rec seq start = function
+| O -> []
+| S len0 -> start :: (seq (S start) len0)
+
+type positive =
+| XI of positive
+| XO of positive
+| XH
+
+type z =
+| Z0
+| Zpos of positive
+| Zneg of positive
+
+module Pos =
+ struct
+  (** val succ : positive -> positive **)
+
+  let rec succ = function
+  | XI p -> XO (succ p)
+  | XO p -> XI p
+  | XH -> XO XH
+
+  (** val add : positive -> positive -> positive **)
+
+  let rec add x y =
+    match x with
+    | XI p ->
+      (match y with
+       | XI q -> XO (add_carry p q)
+       | XO q -> XI (add p q)
+       | XH -> XO (succ p))
+    | XO p ->
+      (match y with
+       | XI q -> XI (add p q)
+       | XO q -> XO (add p q)
+       | XH -> XI p)
+    | XH -> (match y with
+             | XI q -> XO (succ q)
+             | XO q -> XI q
+             | XH -> XO XH)
+
+  (** val add_carry : positive -> positive -> positive **)
+
+  and add_carry x y =
+    match x with
+    | XI p ->
+      (match y with
+       | XI q -> XI (add_carry p q)
+       | XO q -> XO (add_carry p q)
+       | XH -> XI (succ p))
+    | XO p ->
+      (match y with
+       | XI q -> XO (add_carry p q)
+       | XO q -> XI (add p q)
+       | XH -> XO (succ p))
+    | XH ->
+      (match y with
+       | XI q -> XI (succ q)
+       | XO q -> XO (succ q)
+       | XH -> XI XH)
+
+  (** val pred_double : positive -> positive **)
+
+  let rec pred_double = function
+  | XI p -> XI (XO p)
+  | XO p -> XI (pred_double p)
+  | XH -> XH
+
+  (** val mul : positive -> positive -> positive **)
+
+  let rec mul x y =
+    match x with
+    | XI p -> add y (XO (mul p y))
+    | XO p -> XO (mul p y)
+    | XH -> y
+
+  (** val compare_cont : comparison -> positive -> positive -> comparison **)
+
+  let rec compare_cont r x y =
+    match x with
+    | XI p ->
+      (match y with
+       | XI q -> compare_cont r p q
+       | XO q -> compare_cont Gt p q
+       | XH -> Gt)
+    | XO p ->
+      (match y with
+       | XI q -> compare_cont Lt p q
+       | XO q -> compare_cont r p q
+       | XH -> Gt)
+    | XH -> (match y with
+             | XH -> r
+             | _ -> Lt)
+
+  (** val compare : positive -> positive -> comparison **)
+
+  let compare =
+    compare_cont Eq
+
+  (** val eqb : positive -> positive -> bool **)
+
+  let rec eqb p q =
+    match p with
+    | XI p0 -> (match q with
+                | XI q0 -> eqb p0 q0
+                | _ -> false)
+    | XO p0 -> (match q with
+                | XO q0 -> eqb p0 q0
+                | _ -> false)
+    | XH -> (match q with
+             | XH -> true
+             | _ -> false)
+
+  (** val iter_op : ('a1 -> 'a1 -> 'a1) -> positive -> 'a1 -> 'a1 **)
+
+  let rec iter_op op p a =
+    match p with
+    | XI p0 -> op a (iter_op op p0 (op a a))
+    | XO p0 -> iter_op op p0 (op a a)
+    | XH -> a
+
+  (** val to_nat : positive -> nat **)
+
+  let to_nat x =
+    iter_op Coq__1.add x (S O)
+
+  (** val of_succ_nat : nat -> positive **)
+
+  let rec of_succ_nat = function
+  | O -> XH
+  | S x -> succ (of_succ_nat x)
+ end
+
+module Z =
+ struct
+  (** val double : z -> z **)
+
+  let double = function
+  | Z0 -> Z0
+  | Zpos p -> Zpos (XO p)
+  | Zneg p -> Zneg (XO p)
+
+  (** val succ_double : z -> z **)
+
+  let succ_double = function
+  | Z0 -> Zpos XH
+  | Zpos p -> Zpos (XI p)
+  | Zneg p -> Zneg (Pos.pred_double p)
+
+  (** val pred_double : z -> z **)
+
+  let pred_double = function
+  | Z0 -> Zneg XH
+  | Zpos p -> Zpos (Pos.pred_double p)
+  | Zneg p -> Zneg (XI p)
+
+  (** val pos_sub : positive -> positive -> z **)
+
+  let rec pos_sub x y =
+    match x with
+    | XI p ->
+      (match y with
+       | XI q -> double (pos_sub p q)
+       | XO q -> succ_double (pos_sub p q)
+       | XH -> Zpos (XO p))
+    | XO p ->
+      (match y with
+       | XI q -> pred_double (pos_sub p q)
+       | XO q -> double (pos_sub p q)
+       | XH -> Zpos (Pos.pred_double p))
+    | XH ->
+      (match y with
+       | XI q -> Zneg (XO q)
+       | XO q -> Zneg (Pos.pred_double q)
+       | XH -> Z0)
+
+  (** val add : z -> z -> z **)
+
+  let add x y =
+    match x with
+    | Z0 -> y
+    | Zpos x' ->
+      (match y with
+       | Z0 -> x
+       | Zpos y' -> Zpos (Pos.add x' y')
+       | Zneg y' -> pos_sub x' y')
+    | Zneg x' ->
+      (match y with
+       | Z0 -> x
+       | Zpos y' -> pos_sub y' x'
+       | Zneg y' -> Zneg (Pos.add x' y'))
+
+  (** val opp : z -> z **)
+
+  let opp = function
+  | Z0 -> Z0
+  | Zpos x0 -> Zneg x0
+  | Zneg x0 -> Zpos x0
+
+  (** val sub : z -> z -> z **)
+
+  let sub m n =
+    add m (opp n)
+
+  (** val mul : z -> z -> z **)
+
+  let mul x y =
+    match x with
+    | Z0 -> Z0
+    | Zpos x' ->
+      (match y with
+       | Z0 -> Z0
+       | Zpos y' -> Zpos (Pos.mul x' y')
+       | Zneg y' -> Zneg (Pos.mul x' y'))
+    | Zneg x' ->
+      (match y with
+       | Z0 -> Z0
+       | Zpos y' -> Zneg (Pos.mul x' y')
+       | Zneg y' -> Zpos (Pos.mul x' y'))
+
+  (** val compare : z -> z -> comparison **)
+
+  let compare x y =
+    match x with
+    | Z0 -> (match y with
+             | Z0 -> Eq
+             | Zpos _ -> Lt
+             | Zneg _ -> Gt)
+    | Zpos x' -> (match y with
+                  | Zpos y' -> Pos.compare x' y'
+                  | _ -> Gt)
+    | Zneg x' ->
+      (match y with
+       | Zneg y' -> compOpp (Pos.compare x' y')
+       | _ -> Lt)
+
+  (** val leb : z -> z -> bool **)
+
+  let leb x y =
+    match compare x y with
+    | Gt -> false
+    | _ -> true
+
+  (** val ltb : z -> z -> bool **)
+
+  let ltb x y =
+    match compare x y with
+    | Lt -> true
+    | _ -> false
+
+  (** val eqb : z -> z -> bool **)
+
+  let eqb x y =
+    match x with
+    | Z0 -> (match y with
+             | Z0 -> true
+             | _ -> false)
+    | Zpos p -> (match y with
+                 | Zpos q -> Pos.eqb p q
+                 | _ -> false)
+    | Zneg p -> (match y with
+                 | Zneg q -> Pos.eqb p q
+                 | _ -> false)
+
+  (** val to_nat : z -> nat **)
+
+  let to_nat = function
+  | Zpos p -> Pos.to_nat p
+  | _ -> O
+
+  (** val of_nat : nat -> z **)
+
+  let of_nat = function
+  | O -> Z0
+  | S n0 -> Zpos (Pos.of_succ_nat n0)
+
+  (** val pos_div_eucl : positive -> z -> z * z **)
+
+  let rec pos_div_eucl a b =
+    match a with
+    | XI a' ->
+      let (q, r) = pos_div_eucl a' b in
+      let r' = add (mul (Zpos (XO XH)) r) (Zpos XH) in
+      if ltb r' b
+      then ((mul (Zpos (XO XH)) q), r')
+      else ((add (mul (Zpos (XO XH)) q) (Zpos XH)), (sub r' b))
+    | XO a' ->
+      let (q, r) = pos_div_eucl a' b in
+      let r' = mul (Zpos (XO XH)) r in
+      if ltb r' b
+      then ((mul (Zpos (XO XH)) q), r')
+      else ((add (mul (Zpos (XO XH)) q) (Zpos XH)), (sub r' b))
+    | XH -> if leb (Zpos (XO XH)) b then (Z0, (Zpos XH)) else ((Zpos XH), Z0)
+
+  (** val div_eucl : z -> z -> z * z **)
+
+  let div_eucl a b =
+    match a with
+    | Z0 -> (Z0, Z0)
+    | Zpos a' ->
+      (match b with
+       | Z0 -> (Z0, a)
+       | Zpos _ -> pos_div_eucl a' b
+       | Zneg b' ->
+         let (q, r) = pos_div_eucl a' (Zpos b') in
+         (match r with
+          | Z0 -> ((opp q), Z0)
+          | _ -> ((opp (add q (Zpos XH))), (add b r))))
+    | Zneg a' ->
+      (match b with
+       | Z0 -> (Z0, a)
+       | Zpos _ ->
+         let (q, r) = pos_div_eucl a' b in
+         (match r with
+          | Z0 -> ((opp q), Z0)
+          | _ -> ((opp (add q (Zpos XH))), (sub b r)))
+       | Zneg b' -> let (q, r) = pos_div_eucl a' (Zpos b') in (q, (opp r)))
+
+  (** val modulo : z -> z -> z **)
+
+  let modulo a b =
+    let (_, r) = div_eucl a b in r
+ end
+
+(** val eqb0 : char list -> char list -> bool **)
+
+let rec eqb0 s1 s2 =
+  match s1 with
+  | [] -> (match s2 with
+           | [] -> true
+           | _::_ -> false)
+  | c1::s1' ->
+    (match s2 with
+     | [] -> false
+     | c2::s2' -> if (=) c1 c2 then eqb0 s1' s2' else false)
+
+type 'a total_map = char list -> 'a
+
+type 'a partial_map = 'a option total_map
+
+type 'a stream = 'a __stream Lazy.t
+and 'a __stream =
+| Cons of 'a * 'a stream
+
+(** val hd : 'a1 stream -> 'a1 **)
+
+let hd x =
+  let Cons (a, _) = Lazy.force x in a
+
+(** val list_beq : ('a1 -> 'a1 -> bool) -> 'a1 list -> 'a1 list -> bool **)
+
+let rec list_beq eq_A x y =
+  match x with
+  | [] -> (match y with
+           | [] -> true
+           | _ :: _ -> false)
+  | x0 :: x1 ->
+    (match y with
+     | [] -> false
+     | x2 :: x3 -> (&&) (eq_A x0 x2) (list_beq eq_A x1 x3))
+
+type ivytype =
+| Ivytype_Bool
+| Ivytype_User_Defined of char list
+| Ivytype_Fun of ivytype list * ivytype
+| Ivytype_Void
+
+(** val eqb_Ivytype : ivytype -> ivytype -> bool **)
+
+let rec eqb_Ivytype t1 t2 =
+  match t1 with
+  | Ivytype_Bool -> (match t2 with
+                     | Ivytype_Bool -> true
+                     | _ -> false)
+  | Ivytype_User_Defined s1 ->
+    (match t2 with
+     | Ivytype_User_Defined s2 -> eqb0 s1 s2
+     | _ -> false)
+  | Ivytype_Fun (ts1, t3) ->
+    (match t2 with
+     | Ivytype_Fun (ts2, t4) ->
+       (&&) (list_beq eqb_Ivytype ts1 ts2) (eqb_Ivytype t3 t4)
+     | _ -> false)
+  | Ivytype_Void -> (match t2 with
+                     | Ivytype_Void -> true
+                     | _ -> false)
+
+type expr =
+| Expr_VarLiteral of char list
+| Expr_EnumVarLiteral of ivytype * nat
+| Expr_VarFun of char list * expr list
+| Expr_True
+| Expr_False
+| Expr_Not of expr
+| Expr_And of expr * expr
+| Expr_Or of expr * expr
+| Expr_Eq of expr * expr
+| Expr_Implies of expr * expr
+| Expr_Iff of expr * expr
+| Expr_Forall of char list * ivytype * expr
+| Expr_Exists of char list * ivytype * expr
+| Expr_Nondet of ivytype
+| Expr_Cond of expr * expr * expr
+| Expr_Error
+
+(** val eqb_Expr : expr -> expr -> bool **)
+
+let rec eqb_Expr e1 e2 =
+  match e1 with
+  | Expr_VarLiteral x1 ->
+    (match e2 with
+     | Expr_VarLiteral x2 -> eqb0 x1 x2
+     | _ -> false)
+  | Expr_EnumVarLiteral (t1, n1) ->
+    (match e2 with
+     | Expr_EnumVarLiteral (t2, n2) -> (&&) (eqb_Ivytype t1 t2) (eqb n1 n2)
+     | _ -> false)
+  | Expr_VarFun (x1, es1) ->
+    (match e2 with
+     | Expr_VarFun (x2, es2) -> (&&) (eqb0 x1 x2) (list_beq eqb_Expr es1 es2)
+     | _ -> false)
+  | Expr_True -> (match e2 with
+                  | Expr_True -> true
+                  | _ -> false)
+  | Expr_False -> (match e2 with
+                   | Expr_False -> true
+                   | _ -> false)
+  | Expr_Not e3 -> (match e2 with
+                    | Expr_Not e4 -> eqb_Expr e3 e4
+                    | _ -> false)
+  | Expr_And (e11, e12) ->
+    (match e2 with
+     | Expr_And (e21, e22) -> (&&) (eqb_Expr e11 e21) (eqb_Expr e12 e22)
+     | _ -> false)
+  | Expr_Or (e11, e12) ->
+    (match e2 with
+     | Expr_Or (e21, e22) -> (&&) (eqb_Expr e11 e21) (eqb_Expr e12 e22)
+     | _ -> false)
+  | Expr_Eq (e11, e12) ->
+    (match e2 with
+     | Expr_Eq (e21, e22) -> (&&) (eqb_Expr e11 e21) (eqb_Expr e12 e22)
+     | _ -> false)
+  | Expr_Implies (e11, e12) ->
+    (match e2 with
+     | Expr_Implies (e21, e22) -> (&&) (eqb_Expr e11 e21) (eqb_Expr e12 e22)
+     | _ -> false)
+  | Expr_Iff (e11, e12) ->
+    (match e2 with
+     | Expr_Iff (e21, e22) -> (&&) (eqb_Expr e11 e21) (eqb_Expr e12 e22)
+     | _ -> false)
+  | Expr_Nondet t1 ->
+    (match e2 with
+     | Expr_Nondet t2 -> eqb_Ivytype t1 t2
+     | _ -> false)
+  | Expr_Cond (e11, e12, e13) ->
+    (match e2 with
+     | Expr_Cond (e21, e22, e23) ->
+       (&&) (eqb_Expr e11 e21) ((&&) (eqb_Expr e12 e22) (eqb_Expr e13 e23))
+     | _ -> false)
+  | _ -> false
+
+type com =
+| Com_Assign of char list * expr
+| Com_AssignFun of char list * char list list * expr
+| Com_Seq of com * com
+| Com_If of expr * com
+| Com_IfElse of expr * com * com
+| Com_For of char list * ivytype * com
+| Com_While of expr * com
+| Com_LocalVarDecl of char list * ivytype
+| Com_GlobalVarDecl of char list * ivytype
+| Com_GlobalFuncVarDecl of char list * ivytype list * ivytype
+| Com_TypeDecl of char list * nat
+| Com_ActionDecl of char list * (char list * ivytype) list * ivytype * com
+| Com_Skip
+
+(** val is_value : expr -> bool **)
+
+let rec is_value = function
+| Expr_VarLiteral _ -> true
+| Expr_VarFun (_, es) -> fold_left (fun b e0 -> (&&) b (is_value e0)) es true
+| Expr_True -> true
+| Expr_False -> true
+| _ -> false
+
+(** val subst : expr -> expr -> char list -> expr **)
+
+let rec subst e v x =
+  match e with
+  | Expr_VarLiteral y -> if eqb0 x y then v else e
+  | Expr_VarFun (y, es) -> Expr_VarFun (y, (map (fun e0 -> subst e0 v x) es))
+  | Expr_Not e0 -> Expr_Not (subst e0 v x)
+  | Expr_And (e1, e2) -> Expr_And ((subst e1 v x), (subst e2 v x))
+  | Expr_Or (e1, e2) -> Expr_Or ((subst e1 v x), (subst e2 v x))
+  | Expr_Eq (e1, e2) -> Expr_Eq ((subst e1 v x), (subst e2 v x))
+  | Expr_Implies (e1, e2) -> Expr_Implies ((subst e1 v x), (subst e2 v x))
+  | Expr_Iff (e1, e2) -> Expr_Iff ((subst e1 v x), (subst e2 v x))
+  | Expr_Forall (y, t, e0) -> Expr_Forall (y, t, (subst e0 v x))
+  | Expr_Exists (y, t, e0) -> Expr_Exists (y, t, (subst e0 v x))
+  | Expr_Cond (e1, e2, e3) ->
+    Expr_Cond ((subst e1 v x), (subst e2 v x), (subst e3 v x))
+  | x0 -> x0
+
+type context = ivytype partial_map
+
+type enumTypeSizes = ivytype -> nat
+
+type action_context =
+  (((char list * ivytype) list * ivytype) * com) partial_map
+
+(** val fromMaybe : 'a1 -> 'a1 option -> 'a1 **)
+
+let fromMaybe x = function
+| Some z0 -> z0
+| None -> x
+
+(** val rand : z -> z -> z -> z stream **)
+
+let rec rand seed n1 n2 =
+  let seed' = Z.modulo seed n2 in
+  lazy (Cons (seed', (rand (Z.mul seed' n1) n1 n2)))
+
+(** val nondet_helper : ivytype -> enumTypeSizes -> expr option **)
+
+let nondet_helper t type_sizes =
+  match t with
+  | Ivytype_Bool ->
+    if Z.eqb (hd (rand Z0 (Zpos (XO XH)) (Zpos (XI XH)))) Z0
+    then Some Expr_True
+    else Some Expr_False
+  | Ivytype_User_Defined _ ->
+    Some (Expr_EnumVarLiteral (t,
+      (Z.to_nat
+        (hd
+          (rand Z0 (Zpos (XO XH)) (Z.add (Z.of_nat (type_sizes t)) (Zpos XH)))))))
+  | _ -> None
+
+(** val small_step_Expr :
+    expr -> context -> context -> action_context -> (ivytype -> bool) ->
+    enumTypeSizes -> expr option **)
+
+let rec small_step_Expr e var_ctx fun_var_ctx act_ctx declared_types type_sizes =
+  match e with
+  | Expr_VarFun (x, es) ->
+    (match fun_var_ctx x with
+     | Some i ->
+       (match i with
+        | Ivytype_Fun (_, _) ->
+          (match es with
+           | [] -> None
+           | e0 :: es' ->
+             (match small_step_Expr e0 var_ctx fun_var_ctx act_ctx
+                      declared_types type_sizes with
+              | Some e' -> Some (Expr_VarFun (x, (e' :: es')))
+              | None ->
+                (match es' with
+                 | [] -> None
+                 | e' :: es'' ->
+                   (match small_step_Expr e' var_ctx fun_var_ctx act_ctx
+                            declared_types type_sizes with
+                    | Some e'' ->
+                      Some (Expr_VarFun (x, (e0 :: (e'' :: es''))))
+                    | None -> None))))
+        | _ -> None)
+     | None -> None)
+  | Expr_Not e' ->
+    if is_value e'
+    then (match e' with
+          | Expr_True -> Some Expr_False
+          | Expr_False -> Some Expr_True
+          | _ -> None)
+    else let e'' =
+           small_step_Expr e' var_ctx fun_var_ctx act_ctx declared_types
+             type_sizes
+         in
+         Some (Expr_Not (fromMaybe Expr_Error e''))
+  | Expr_And (e1, e2) ->
+    if is_value e1
+    then if is_value e2
+         then (match e1 with
+               | Expr_True ->
+                 (match e2 with
+                  | Expr_True -> Some Expr_True
+                  | Expr_False -> Some Expr_False
+                  | _ -> None)
+               | Expr_False ->
+                 (match e2 with
+                  | Expr_True -> Some Expr_False
+                  | Expr_False -> Some Expr_False
+                  | _ -> None)
+               | _ -> None)
+         else Some (Expr_And (e1,
+                (fromMaybe Expr_Error
+                  (small_step_Expr e2 var_ctx fun_var_ctx act_ctx
+                    declared_types type_sizes))))
+    else Some (Expr_And
+           ((fromMaybe Expr_Error
+              (small_step_Expr e1 var_ctx fun_var_ctx act_ctx declared_types
+                type_sizes)), e2))
+  | Expr_Or (e1, e2) ->
+    if is_value e1
+    then if is_value e2
+         then (match e1 with
+               | Expr_True ->
+                 (match e2 with
+                  | Expr_True -> Some Expr_True
+                  | Expr_False -> Some Expr_True
+                  | _ -> None)
+               | Expr_False ->
+                 (match e2 with
+                  | Expr_True -> Some Expr_True
+                  | Expr_False -> Some Expr_False
+                  | _ -> None)
+               | _ -> None)
+         else Some (Expr_Or (e1,
+                (fromMaybe Expr_Error
+                  (small_step_Expr e2 var_ctx fun_var_ctx act_ctx
+                    declared_types type_sizes))))
+    else Some (Expr_Or
+           ((fromMaybe Expr_Error
+              (small_step_Expr e1 var_ctx fun_var_ctx act_ctx declared_types
+                type_sizes)), e2))
+  | Expr_Eq (e1, e2) ->
+    if is_value e1
+    then if is_value e2
+         then if eqb_Expr e1 e2 then Some Expr_True else Some Expr_False
+         else Some (Expr_Eq (e1,
+                (fromMaybe Expr_Error
+                  (small_step_Expr e2 var_ctx fun_var_ctx act_ctx
+                    declared_types type_sizes))))
+    else Some (Expr_Eq
+           ((fromMaybe Expr_Error
+              (small_step_Expr e1 var_ctx fun_var_ctx act_ctx declared_types
+                type_sizes)), e2))
+  | Expr_Implies (e1, e2) ->
+    if is_value e1
+    then if is_value e2
+         then (match e1 with
+               | Expr_True ->
+                 (match e2 with
+                  | Expr_True -> Some Expr_True
+                  | Expr_False -> Some Expr_False
+                  | _ -> None)
+               | Expr_False ->
+                 (match e2 with
+                  | Expr_True -> Some Expr_True
+                  | Expr_False -> Some Expr_True
+                  | _ -> None)
+               | _ -> None)
+         else Some (Expr_Implies (e1,
+                (fromMaybe Expr_Error
+                  (small_step_Expr e2 var_ctx fun_var_ctx act_ctx
+                    declared_types type_sizes))))
+    else Some (Expr_Implies
+           ((fromMaybe Expr_Error
+              (small_step_Expr e1 var_ctx fun_var_ctx act_ctx declared_types
+                type_sizes)), e2))
+  | Expr_Iff (e1, e2) ->
+    if is_value e1
+    then if is_value e2
+         then if eqb_Expr e1 e2 then Some Expr_True else Some Expr_False
+         else Some (Expr_Iff (e1,
+                (fromMaybe Expr_Error
+                  (small_step_Expr e2 var_ctx fun_var_ctx act_ctx
+                    declared_types type_sizes))))
+    else Some (Expr_Iff
+           ((fromMaybe Expr_Error
+              (small_step_Expr e1 var_ctx fun_var_ctx act_ctx declared_types
+                type_sizes)), e2))
+  | Expr_Forall (x, t, e') ->
+    let nums = seq O (type_sizes t) in
+    let out =
+      fold_left (fun acc y -> Expr_And (acc,
+        (subst e' (Expr_EnumVarLiteral (t, y)) x))) nums Expr_True
+    in
+    Some out
+  | Expr_Exists (x, t, e') ->
+    let out =
+      fold_left (fun acc y -> Expr_Or (acc,
+        (subst e' (Expr_EnumVarLiteral (t, y)) x))) (seq O (type_sizes t))
+        Expr_False
+    in
+    Some out
+  | Expr_Nondet t -> nondet_helper t type_sizes
+  | Expr_Cond (e1, e2, e3) ->
+    if is_value e1
+    then (match e1 with
+          | Expr_True -> Some e2
+          | Expr_False -> Some e3
+          | _ -> None)
+    else Some (Expr_Cond
+           ((fromMaybe Expr_Error
+              (small_step_Expr e1 var_ctx fun_var_ctx act_ctx declared_types
+                type_sizes)), e2, e3))
+  | _ -> None
