ocaml/generated/extract.mli
@@ -1,0 +1,171 @@
+
+type nat =
+| O
+| S of nat
+
+type comparison =
+| Eq
+| Lt
+| Gt
+
+val compOpp : comparison -> comparison
+
+val add : nat -> nat -> nat
+
+val eqb : nat -> nat -> bool
+
+val map : ('a1 -> 'a2) -> 'a1 list -> 'a2 list
+
+val fold_left : ('a1 -> 'a2 -> 'a1) -> 'a2 list -> 'a1 -> 'a1
+
+val seq : nat -> nat -> nat list
+
+type positive =
+| XI of positive
+| XO of positive
+| XH
+
+type z =
+| Z0
+| Zpos of positive
+| Zneg of positive
+
+module Pos :
+ sig
+  val succ : positive -> positive
+
+  val add : positive -> positive -> positive
+
+  val add_carry : positive -> positive -> positive
+
+  val pred_double : positive -> positive
+
+  val mul : positive -> positive -> positive
+
+  val compare_cont : comparison -> positive -> positive -> comparison
+
+  val compare : positive -> positive -> comparison
+
+  val eqb : positive -> positive -> bool
+
+  val iter_op : ('a1 -> 'a1 -> 'a1) -> positive -> 'a1 -> 'a1
+
+  val to_nat : positive -> nat
+
+  val of_succ_nat : nat -> positive
+ end
+
+module Z :
+ sig
+  val double : z -> z
+
+  val succ_double : z -> z
+
+  val pred_double : z -> z
+
+  val pos_sub : positive -> positive -> z
+
+  val add : z -> z -> z
+
+  val opp : z -> z
+
+  val sub : z -> z -> z
+
+  val mul : z -> z -> z
+
+  val compare : z -> z -> comparison
+
+  val leb : z -> z -> bool
+
+  val ltb : z -> z -> bool
+
+  val eqb : z -> z -> bool
+
+  val to_nat : z -> nat
+
+  val of_nat : nat -> z
+
+  val pos_div_eucl : positive -> z -> z * z
+
+  val div_eucl : z -> z -> z * z
+
+  val modulo : z -> z -> z
+ end
+
+val eqb0 : char list -> char list -> bool
+
+type 'a total_map = char list -> 'a
+
+type 'a partial_map = 'a option total_map
+
+type 'a stream = 'a __stream Lazy.t
+and 'a __stream =
+| Cons of 'a * 'a stream
+
+val hd : 'a1 stream -> 'a1
+
+val list_beq : ('a1 -> 'a1 -> bool) -> 'a1 list -> 'a1 list -> bool
+
+type ivytype =
+| Ivytype_Bool
+| Ivytype_User_Defined of char list
+| Ivytype_Fun of ivytype list * ivytype
+| Ivytype_Void
+
+val eqb_Ivytype : ivytype -> ivytype -> bool
+
+type expr =
+| Expr_VarLiteral of char list
+| Expr_EnumVarLiteral of ivytype * nat
+| Expr_VarFun of char list * expr list
+| Expr_True
+| Expr_False
+| Expr_Not of expr
+| Expr_And of expr * expr
+| Expr_Or of expr * expr
+| Expr_Eq of expr * expr
+| Expr_Implies of expr * expr
+| Expr_Iff of expr * expr
+| Expr_Forall of char list * ivytype * expr
+| Expr_Exists of char list * ivytype * expr
+| Expr_Nondet of ivytype
+| Expr_Cond of expr * expr * expr
+| Expr_Error
+
+val eqb_Expr : expr -> expr -> bool
+
+type com =
+| Com_Assign of char list * expr
+| Com_AssignFun of char list * char list list * expr
+| Com_Seq of com * com
+| Com_If of expr * com
+| Com_IfElse of expr * com * com
+| Com_For of char list * ivytype * com
+| Com_While of expr * com
+| Com_LocalVarDecl of char list * ivytype
+| Com_GlobalVarDecl of char list * ivytype
+| Com_GlobalFuncVarDecl of char list * ivytype list * ivytype
+| Com_TypeDecl of char list * nat
+| Com_ActionDecl of char list * (char list * ivytype) list * ivytype * com
+| Com_Skip
+
+val is_value : expr -> bool
+
+val subst : expr -> expr -> char list -> expr
+
+type context = ivytype partial_map
+
+type enumTypeSizes = ivytype -> nat
+
+type action_context =
+  (((char list * ivytype) list * ivytype) * com) partial_map
+
+val fromMaybe : 'a1 -> 'a1 option -> 'a1
+
+val rand : z -> z -> z -> z stream
+
+val nondet_helper : ivytype -> enumTypeSizes -> expr option
+
+val small_step_Expr :
+  expr -> context -> context -> action_context -> (ivytype -> bool) ->
+  enumTypeSizes -> expr option
